cava/Cava/Acorn/SequentialV.v
@@ -33,6 +33,7 @@ From Coq Require Import micromega.Lia.
 
 Require Import Cava.Cava.
 Require Import Cava.Acorn.CavaClass.
+Require Import Cava.Acorn.CavaPrelude.
 Require Import Cava.Acorn.CombinationalMonad.
 
 Local Open Scope vector_scope.
@@ -89,7 +90,7 @@ to compute the sequential behaviour of a circuit which uses f to iterate over
 the a inputs, using a default value for the initial state.
  *)
 
-Definition loopSeqSV {A B : SignalType} (ticks : nat)
+Definition loopSeqSV {A B : SignalType} (ticks : nat) (resetval : combType B)
   : (seqVType ticks A * seqVType ticks B -> ident (seqVType ticks B))
     -> seqVType ticks A -> ident (seqVType ticks B) :=
   match ticks as ticks0 return
@@ -98,8 +99,7 @@ Definition loopSeqSV {A B : SignalType} (ticks : nat)
   | O => fun _ _ => ret []
   | S ticks' =>
     fun f a =>
-      loopSeqSV' (S ticks') (stepOnce f)
-                a [defaultCombValue B]
+      loopSeqSV' (S ticks') (stepOnce f) a [resetval]
   end.
 
 (******************************************************************************)
@@ -224,10 +224,10 @@ Definition bufBoolVec (ticks: nat)
            (i : Vector.t bool ticks) : ident (Vector.t bool ticks) :=
   ret i.
 
-Definition delayV (ticks : nat) (t : SignalType) : seqVType ticks t -> ident (seqVType ticks t) :=
+Definition delayV (ticks : nat) (t : SignalType) (def : combType t) : seqVType ticks t -> ident (seqVType ticks t) :=
   match ticks as ticks0 return seqVType ticks0 t -> ident (seqVType ticks0 t) with
   | O => fun _ => ret []
-  | S ticks' => fun i => ret (defaultCombValue t :: Vector.shiftout i)
+  | S ticks' => fun i => ret (def  :: Vector.shiftout i)
   end.
 
 (******************************************************************************)
@@ -272,16 +272,16 @@ Definition delayV (ticks : nat) (t : SignalType) : seqVType ticks t -> ident (se
 
  Instance SequentialVectorSemantics {ticks: nat}
    : CavaSeq SequentialVectorCombSemantics:=
-   { delay k i := delayV ticks k i;
+   { delayWith k d i := delayV ticks k d i;
      (* Dummy definition now for delayEnable.
         TODO(satnam6502, jadephilipoom): implement delayEnableV
      *)
-     delayEnable k en i := delayV ticks k i;
-     loopDelayS A B := @loopSeqSV A B ticks;
+     delayEnableWith k d en i := delayV ticks k d i;
+     loopDelaySR A B := @loopSeqSV A B ticks;
      (* TODO(satnam6502, jadep): Placeholder definition for loopDelayEnable for
         now. Replace with actual definition that models clock enable behaviour.
      *)
-     loopDelaySEnable A B en := @loopSeqSV A B ticks; (* Dummy *)
+     loopDelaySEnableR A B resetval en := @loopSeqSV A B ticks resetval; (* Dummy *)
    }.
 
 (******************************************************************************)
